Overhaul of EverCrypt.CRF
- Switch to a stateful state.
- Add a run-time representation of the algorithm for finish.
- Everything else takes an erased algorithm.
- Figure out all the right disjointness preconditions for the TLS tables
  region.
- Write helpers to minimize the pain dealing with idealized types.
- Introduce a dependent pair for the model state.
- Write enough helpers that the rest of the module is almost a
  copy-paste of EverCrypt.Hash.Incremental.

src/tls/EverCrypt.CRF.fst
@@ -1,70 +1,87 @@
 module EverCrypt.CRF
 
 module Concrete = EverCrypt.Hash.Incremental
-module Hash = EverCrypt.Hash 
+module Hash = EverCrypt.Hash
 
 module B = LowStar.Buffer
 module ST = FStar.HyperStack.ST
 module HS = FStar.HyperStack
 
-open FStar.HyperStack.ST 
+open FStar.HyperStack.ST
 
 /// migrate these 2 functions to no_extract LowStar.Buffer?
-/// 
-assume val to_seq 
-  (#a:Type0) 
-  // (#rrel #rel:B.srel a) 
+///
+assume val to_seq
+  (#a:Type0)
+  // (#rrel #rel:B.srel a)
   // (b:B.mbuffer a rrel rel)
   (b: B.buffer a)
   (l:UInt32.t {UInt32.v l == B.length b})
-  : 
+  :
   Stack (Seq.seq a)
     (fun h0 -> B.live h0 b)
-    (fun h0 s h1 -> 
+    (fun h0 s h1 ->
       h0 == h1 /\
       B.as_seq h0 b == s )
 
-assume val of_seq 
-  (#a:Type0) 
-  // (#rrel #rel:B.srel a) 
+assume val of_seq
+  (#a:Type0)
+  // (#rrel #rel:B.srel a)
   // (b:B.mbuffer a rrel rel)
   (b: B.buffer a)
-  (s: Seq.seq a) 
-  : 
+  (s: Seq.seq a)
+  :
   Stack unit
-    (fun h0 -> 
-      B.live h0 b /\ 
+    (fun h0 ->
+      B.live h0 b /\
       B.length b = Seq.length s)
-    (fun h0 _ h1 -> 
+    (fun h0 _ h1 ->
       B.modifies (B.loc_buffer b) h0 h1 /\
       B.as_seq h1 b == s)
 
-
-let create_in a r = 
-  if model then 
-    Seq.empty <: mstate 
-    // (B.malloc r (Seq.empty <: bytes) 1ul <: mstate) <: state a
+let create_in a r =
+  if model then
+    let s = B.malloc r (Seq.empty <: bytes) 1ul in
+    ((| a, s |) <: mstate a) <: state a
   else
-    Concrete.create_in a r 
+    Concrete.create_in a r
 
-let update a s prev data len = 
-  if model then 
-    Seq.append s (to_seq data len)
-    // B.upd (s <: mstate) 0ul (Seq.append (B.index (s <: mstate) 0ul) delta)
+let init a s =
+  let open LowStar.BufferOps in
+  if model then
+    let s: B.pointer bytes = snd s in
+    s *= S.empty
   else
-    Concrete.update a s prev data len 
+    Concrete.init a s
 
-#set-options "--z3rlimit 100" 
-let finish a s prev dst = 
-  assert_norm(pow2 61 < pow2 125);
-  assert(Model.CRF.hashable (Ghost.reveal prev));
-  assert(Seq.length (Ghost.reveal prev) < Hash.maxLength a);
-  if model then 
-    let tag = Model.CRF.hash a s in
-    dst `of_seq` tag
-  else (
-    Model.CRF.concrete_hashed a (Ghost.reveal prev);
-    Concrete.finish a s prev dst)
-    
-let free a s = if model then () else Concrete.free a s
-    
+let update a s data len =
+  let open LowStar.BufferOps in
+  if model then
+    let s: B.pointer bytes = snd s in
+    s *= (S.append !*s (to_seq data len))
+  else
+    Concrete.update a s data len
+
+#push-options "--z3rlimit 50"
+let finish a st dst =
+  let open LowStar.BufferOps in
+  if model then
+    let a = fst #a st in
+    let s: B.pointer bytes = snd st in
+    (**) assert B.(loc_disjoint (B.loc_addr_of_buffer s)
+      (B.loc_region_only true Mem.tls_tables_region));
+    (**) let h0 = ST.get () in
+    let hash = Model.CRF.hash a !*s in
+    (**) let h1 = ST.get () in
+    (**) assert (B.live h1 dst);
+    (**) frame_invariant #a (B.loc_region_only true Mem.tls_tables_region) st h0 h1;
+    dst `of_seq` hash
+  else
+    Concrete.finish a st dst
+
+let free a s =
+  if model then
+    B.free (snd s)
+  else
+    Concrete.free a s
+
