src/tls/EverCrypt.CRF.fsti
@@ -3,181 +3,288 @@ module EverCrypt.CRF
 /// Status. See also `Test.CRF.fst`.
 ///
 /// * Relocate to EverCrypt? But we depend on mitls flags.
-/// 
+///
 /// * Still relies on `FStar.Monotonic.DependentMap`, not clearly
 ///   compatible with location-based modifies and Stack. For now I am
 ///   assuming a modifies clause. But we need to find a style where we
 ///   can modify the TLS region without too much trouble.
-///
-/// * This suggests improvements to the incremental interface (see comments in the files).
-///
-/// * We should make the incremental-state abstract: this is required
-///   for the `switch` step, and may help with verification speed.
 
 module Concrete = EverCrypt.Hash.Incremental
-module Hash = EverCrypt.Hash 
+module Hash = EverCrypt.Hash
 
 module B = LowStar.Buffer
 module ST = FStar.HyperStack.ST
 module HS = FStar.HyperStack
+module S = FStar.Seq
+module U32 = FStar.UInt32
+module G = FStar.Ghost
 
-open FStar.HyperStack.ST 
+open FStar.HyperStack.ST
 
-let model = Flags.model 
-// not sure where to put the flags, or if we need a separate one 
+let model = Flags.model
+// not sure where to put the flags, or if we need a separate one
 
 /// We first switch to a (non-extracted) implementation of the
 /// EverCrypt.Hash.Incremental API that accumulates the text to hash
 /// it using the pure spec only at extraction-time. When model=false,
 /// the two implementations share the same full specs.
+///
+/// JP: Note that the state is not abstract, i.e. we don't re-add another layer
+/// of abstraction with framing lemmas. Should we?
 
-// TODO test that verification usability matches Concrete. 
-// TODO refactor EverCrypt to make such switches less verbose? 
+// TODO test that verification usability matches Concrete.
+// TODO refactor EverCrypt to make such switches less verbose?
 // TODO make the state abstract---requires pre/post rewriting
 // TODO hide Model, treating hashed as an abstract predicate. Confirm we don't import algorithmic specs.
 
-let bytes = Model.CRF.bytes 
-let hashed = Model.CRF.hashed 
-//type hashable = b:bytes {Model.CRF.hashable b}
+#set-options "--max_fuel 0 --max_ifuel 0"
 
-type mstate = bytes // hashable 
-// tried first a stateful variant, unnecessary since Concrete is
-// actually state-passing.
-// type mstate = b:B.buffer hashable {B.length b = 1}
+/// Re-exporting all the definitions with a switch
+/// ----------------------------------------------
 
-let state (a:Hash.alg) = if model then mstate else Concrete.state a
+unfold noextract
+let bytes = Model.CRF.bytes
 
-let footprint #a (s: state a) h = 
-  if model then 
-    B.loc_none // B.loc_addr_of_buffer (s <: mstate)
-  else 
-    Concrete.footprint #a s h // (s <: Concrete.state a) h
-  
-let freeable #a (s:state a) h = 
-  if model then True else Concrete.freeable #a s h
+unfold noextract
+let e_alg = Concrete.e_alg
 
-let preserves_freeable #a (s: state a) (h0 h1: HS.mem) = 
-  if model then True else Concrete.preserves_freeable #a s h0 h1
+unfold noextract
+let fresh_loc = Concrete.fresh_loc
 
-let modifies_disjoint_preserves #a (l: B.loc) (h0 h1: HS.mem) (s: state a): Lemma 
-  (requires (
-    B.modifies l h0 h1 /\
-    B.loc_disjoint l (footprint #a s h0) /\ ( 
-    if model then True else 
-      let hash_state = Concrete.State?.hash_state #a s in
-      Hash.invariant #a hash_state h0)))
-  (ensures (
-    footprint #a s h0 == footprint #a s h1 /\ (
-    if model then True else 
-      let hash_state = Concrete.State?.hash_state #a s in
-      Hash.invariant #a hash_state h1 /\
-      Hash.repr #a hash_state h1 == Hash.repr #a hash_state h0 
-      )))
+/// Overriding things
+/// -----------------
+
+/// This is very finely tuned to avoid inference issues.
+type mstate a = a': Concrete.alg { a' == a } & p:B.pointer bytes {
+  B.(loc_disjoint (loc_addr_of_buffer p) (loc_region_only true Mem.tls_tables_region))
+}
+
+let state (a: Concrete.alg) =
+  if model then
+    mstate a
+  else
+    Concrete.state a
+
+// UGH!!!
+noextract inline_for_extraction
+let fst (#a: e_alg) (s: state (G.reveal a){model}):
+  Tot (a': Concrete.alg { G.reveal a == a' })
 =
-  if model then () else Concrete.modifies_disjoint_preserves #a l h0 h1 s
+  if model then
+    let (| a, s |) = (s <: mstate (G.reveal a)) in
+    a
+  else
+    false_elim ()
 
-// #set-options "--max_fuel 0 --max_ifuel 0"
-unfold
-let hashes (#a: Hash.alg) (h: HS.mem) (s: state a) (b: bytes) =
-  Seq.length b < pow2 61 /\ (
-  if model then (
-    Seq.equal s b 
-    // B.live h (s <: mstate) /\
-    // Seq.equal (B.get h (s <: mstate) 0) b
-    )
-  else 
-    Concrete.hashes #a h s b ) 
+noextract inline_for_extraction
+let snd (#a: e_alg) (s: state (G.reveal a){model}):
+  Tot (p:B.pointer bytes {
+    B.(loc_disjoint (loc_addr_of_buffer p) (loc_region_only true Mem.tls_tables_region))
+  })
+=
+  if model then
+    let (| a, s |) = (s <: mstate (G.reveal a)) in
+    s
+  else
+    false_elim ()
 
+let freeable #a h (s:state a) =
+  if model then
+    let s: B.pointer bytes = snd #(G.hide a) s in
+    B.freeable s
+  else
+    Concrete.freeable #a h s
+
+let preserves_freeable #a (s: state a) (h0 h1: HS.mem) =
+  freeable h0 s ==> freeable h1 s
+
+let footprint #a h (s: state a) =
+  if model then
+    B.loc_addr_of_buffer (snd #(G.hide a) s)
+  else
+    Concrete.footprint #a h s
+
+let invariant #a h (s: state a) =
+  if model then
+    let s: B.pointer bytes = snd #(G.hide a) s in
+    B.live h s /\ S.length (B.deref h s) < pow2 61
+  else
+    Concrete.invariant #a h s
+
+let invariant_loc_in_footprint
+  (#a: Concrete.alg)
+  (s: state a)
+  (m: HS.mem)
+: Lemma
+  (requires (invariant m s))
+  (ensures (Concrete.loc_in (footprint m s) m))
+  [SMTPat (invariant m s)]
+=
+  ()
+
+let hashed #a h (s: state a) =
+  if model then
+    let s: B.pointer bytes = snd #(G.hide a) s in
+    B.deref h s
+  else
+    let s: Concrete.state a = s in
+    Concrete.hashed h s
+
+#push-options "--max_ifuel 1"
+let hash_fits (#a:Hash.alg) (h:HS.mem) (s:state a): Lemma
+  (requires (
+    invariant h s))
+  (ensures (
+    S.length (hashed h s) < Spec.Hash.Definitions.max_input_length a))
+  [ SMTPat (hashed h s) ]
+=
+  assert_norm (pow2 61 < pow2 125);
+  ()
+#pop-options
+
+let frame_invariant (#a: Concrete.alg) (l: B.loc) (s: state a) (h0 h1: HS.mem): Lemma
+  (requires (
+    invariant h0 s /\
+    B.loc_disjoint l (footprint h0 s) /\
+    B.modifies l h0 h1))
+  (ensures (
+    invariant h1 s /\
+    footprint h0 s == footprint h1 s))
+  [ SMTPat (invariant h1 s); SMTPat (B.modifies l h0 h1) ]
+=
+  ()
+
+let frame_hashed (#a: Concrete.alg) (l: B.loc) (s: state a) (h0 h1: HS.mem): Lemma
+  (requires (
+    invariant h0 s /\
+    B.loc_disjoint l (footprint h0 s) /\
+    B.modifies l h0 h1))
+  (ensures (hashed h0 s == hashed h1 s))
+  [ SMTPat (hashed h1 s); SMTPat (B.modifies l h0 h1) ]
+=
+  ()
+
+let frame_freeable (#a: Concrete.alg) (l: B.loc) (s: state a) (h0 h1: HS.mem): Lemma
+  (requires (
+    invariant h0 s /\
+    freeable h0 s /\
+    B.loc_disjoint l (footprint h0 s) /\
+    B.modifies l h0 h1))
+  (ensures (freeable h1 s))
+  [ SMTPat (freeable h1 s); SMTPat (B.modifies l h0 h1) ]
+=
+  ()
+
+/// Stateful API
+/// ------------
+
+(** @type: true
+*)
 val create_in (a: Hash.alg) (r: HS.rid): ST (state a)
   (requires (fun _ ->
+    // NEW! ↓
+    B.(loc_disjoint (loc_region_only true r) (loc_region_only true Mem.tls_tables_region)) /\
     HyperStack.ST.is_eternal_region r))
   (ensures (fun h0 s h1 ->
-    hashes h1 s Seq.empty /\
+    invariant h1 s /\
+    hashed h1 s == S.empty /\
     B.(modifies loc_none h0 h1) /\
-    Hash.fresh_loc (footprint s h1) h0 h1 /\
-    B.(loc_includes (loc_region_only true r) (footprint s h1)) /\
-    freeable s h1))
+    fresh_loc (footprint h1 s) h0 h1 /\
+    B.(loc_includes (loc_region_only true r) (footprint h1 s)) /\
+    freeable h1 s))
+
+(** @type: true
+*)
+val init: a:e_alg -> (
+  let a = G.reveal a in
+  s:state a -> Stack unit
+  (requires (fun h0 ->
+    invariant h0 s))
+  (ensures (fun h0 _ h1 ->
+    preserves_freeable s h0 h1 /\
+    invariant h1 s /\
+    hashed h1 s == S.empty /\
+    footprint h0 s == footprint h1 s /\
+    B.(modifies (footprint h0 s) h0 h1))))
 
 unfold
 let update_pre
   (a: Hash.alg)
   (s: state a)
-  (prev: Ghost.erased bytes)
   (data: B.buffer UInt8.t)
   (len: UInt32.t)
   (h0: HS.mem)
 =
-  hashes h0 s (Ghost.reveal prev) /\
+  invariant h0 s /\
   B.live h0 data /\
-  UInt32.v len = B.length data /\
-  Seq.length (Ghost.reveal prev) + UInt32.v len < pow2 61 /\
-  B.(loc_disjoint (loc_buffer data) (footprint s h0))
+  U32.v len = B.length data /\
+  S.length (hashed h0 s) + U32.v len < pow2 61 /\
+  B.(loc_disjoint (loc_buffer data) (footprint h0 s))
 
 unfold
 let update_post
   (a: Hash.alg)
-  (s s': state a)
-  (prev: Ghost.erased bytes)
+  (s: state a)
   (data: B.buffer UInt8.t)
   (len: UInt32.t)
   (h0 h1: HS.mem)
 =
-  B.(modifies (footprint s h0) h0 h1) /\
-  footprint s h0 == footprint s' h1 /\
-  hashes h1 s' (Seq.append (Ghost.reveal prev) (B.as_seq h0 data)) /\
-  preserves_freeable s h0 h1 /\ (
-  if model then 
-    True 
-  else 
-    Concrete.State?.hash_state #a s == Concrete.State?.hash_state #a s' /\
-    Concrete.State?.buf #a s == Concrete.State?.buf #a s' )
+  preserves_freeable s h0 h1 /\
+  invariant h1 s /\
+  B.(modifies (footprint h0 s) h0 h1) /\
+  footprint h0 s == footprint h1 s /\
+  hashed h1 s == hashed h0 s `S.append` B.as_seq h0 data
 
+(** @type: true
+*)
 val update:
-  a:Hash.alg ->
+  a:e_alg -> (
+  let a = G.reveal a in
   s:state a ->
-  prev:Ghost.erased bytes ->
   data: B.buffer UInt8.t ->
   len: UInt32.t ->
-  Stack (state a)
-    (requires fun h0 -> update_pre a s prev data len h0)
-    (ensures fun h0 s' h1 -> update_post a s s' prev data len h0 h1)
+  Stack unit
+    (requires fun h0 -> update_pre a s data len h0)
+    (ensures fun h0 s' h1 -> update_post a s data len h0 h1))
 
+/// Note: the state is left to be reused by the caller to feed more data into
+/// the hash.
 inline_for_extraction
 let finish_st (a: Hash.alg) =
   s:state a ->
-  prev:Ghost.erased bytes ->
   dst: Hacl.Hash.Definitions.hash_t a ->
-  Stack unit
+  // NEW! ↓ constrained to ST because Model.CRF.hash (fix MDM?)
+  ST unit
     (requires fun h0 ->
-      hashes h0 s (Ghost.reveal prev) /\
+      invariant h0 s /\
       B.live h0 dst /\
-      B.(loc_disjoint (loc_buffer dst) (footprint s h0)))
+      B.(loc_disjoint (loc_buffer dst) (footprint h0 s)) /\
+      // NEW! ↓
+      B.(loc_disjoint (loc_buffer dst) (loc_region_only true Mem.tls_tables_region)))
     (ensures fun h0 s' h1 ->
-      let text = Ghost.reveal prev in 
-      assert_norm (pow2 61 < pow2 125);
-      hashes h1 s (Ghost.reveal prev) /\
       preserves_freeable s h0 h1 /\
-      footprint s h0 == footprint s h1 /\
-      B.(modifies (loc_union (loc_buffer dst) (footprint s h0)) h0 h1) /\
-      Seq.equal (B.as_seq h1 dst) (Spec.Hash.hash a text) /\
-      (*new*)
-      hashed a text 
-      )
+      invariant h1 s /\
+      hashed h0 s == hashed h1 s /\
+      footprint h0 s == footprint h1 s /\
+      // NEW! ↓
+      B.(modifies (loc_buffer dst `loc_union`
+        footprint h0 s `loc_union`
+        loc_region_only true Mem.tls_tables_region) h0 h1) /\
+      S.equal (B.as_seq h1 dst) (Spec.Hash.hash a (hashed h0 s)))
 
-val finish: a:Hash.alg -> finish_st a
+(** @type: true
+*)
+val finish: a:e_alg -> finish_st (G.reveal a)
 
-val free: 
-  a:Hash.alg ->
-  s:state a -> 
+(** @type: true
+*)
+val free:
+  a:e_alg -> (
+  let a = G.reveal a in
+  s:state a ->
   ST unit
   (requires fun h0 ->
-    freeable s h0 /\ (
-    if model then 
-      True
-    else (
-      let Concrete.State hash_state buf_ _ = (s <: Concrete.state a) in
-      B.live h0 buf_ /\
-      B.(loc_disjoint (loc_buffer buf_) (Hash.footprint hash_state h0)) /\
-      Hash.invariant hash_state h0)))
+    freeable h0 s /\
+    invariant h0 s)
   (ensures fun h0 _ h1 ->
-    B.modifies (footprint s h0) h0 h1)
+    B.modifies (footprint h0 s) h0 h1))
