src/tls/Model.CRF.fst
@@ -1,18 +1,20 @@
 ﻿(** computational assumption: collision resistance *)
 module Model.CRF
 
-/// This module should not be extracted 
+/// This module should not be extracted
 
-open EverCrypt.Hash // only for the specs (renamings)
+open EverCrypt.Hash.Incremental // only for the specs (renamings)
+
+#set-options "--max_fuel 0 --max_ifuel 0"
 
 //2018.04.24 SZ: to be moved elsewhere, set to false for real extraction
 //inline_for_extraction
 // let crf _ = false
-noextract 
+noextract
 assume val crf: alg -> Tot bool
 
-noextract 
-let h = Spec.Hash.hash 
+noextract
+let h = Spec.Hash.hash
 
 (* Depending on a single, global idealization function, we keep a global
     inverse table for all (finalized) hash computations, and we use it to
@@ -21,33 +23,33 @@ let h = Spec.Hash.hash
     This may depend on some prior flag to keep the hashed input in the
     incremental hash implementation. (This is always the case for now.)  *)
 
-open Mem 
-module MDM = FStar.Monotonic.DependentMap 
+open Mem
+module MDM = FStar.Monotonic.DependentMap
 
 // now bounded irrespective of a, as in EverCrypt.Incremental (TBD)
-noextract 
+noextract
 let bytes = Seq.seq UInt8.t
 
 //$ avoid using it because ghost lack structural subtyping.
-noextract 
+noextract
 let hashable (s:bytes) = Seq.length s < pow2 61
 // type hashable (a:alg) = v:Seq.seq UInt8.t {Seq.length v < maxLength a}
 
 // the precise types guarantee that the table stays empty when crf _ = false
-noextract 
-private type range = | Computed: a: alg {crf a} -> t: tag a -> range
+noextract
+private type range = | Computed: a: alg {crf a} -> t: bytes_hash a -> range
 
-noextract 
+noextract
 private type domain (r:range) =
   b:Seq.seq UInt8.t {
-    let Computed a t = r in 
-    Seq.length b < maxLength a /\ 
+    let Computed a t = r in
+    Seq.length b < max_input_length a /\
     h a b = t}
 
-noextract 
+noextract
 private let inv (f:MDM.partial_dependent_map range domain) = True // a bit overkill?
 
-noextract 
+noextract
 private let table : MDM.t tls_tables_region range domain inv = MDM.alloc()
 
 // witnessing that we hashed this particular content (for collision detection)
@@ -56,27 +58,27 @@ private let table : MDM.t tls_tables_region range domain inv = MDM.alloc()
 
 //val hashed: a:alg -> b:bytes -> Type
 
-noextract 
+noextract
 abstract type hashed (a:alg) (b:bytes) =
   model /\ crf a ==> (
     hashable b /\
-    Seq.length b < maxLength a /\
+    Seq.length b < max_input_length a /\
     (
     let t = h a b in
     witnessed (MDM.contains table (Computed a t) (b <: domain (Computed a t)))))
 
-// required to go through abstraction when switching 
-noextract 
+// required to go through abstraction when switching
+noextract
 let concrete_hashed a b: Lemma (~model ==> hashed a b) = ()
 
-val injective (a:alg) (b0 b1: Ghost.erased bytes): 
-  Stack unit  
-  (requires fun h0 -> 
-    let b0 = Ghost.reveal b0 in 
+val injective (a:alg) (b0 b1: Ghost.erased bytes):
+  Stack unit
+  (requires fun h0 ->
+    let b0 = Ghost.reveal b0 in
     let b1 = Ghost.reveal b1 in
     hashed a b0 /\ hashed a b1)
-  (ensures fun h0 _ h1 -> 
-    let b0 = Ghost.reveal b0 in 
+  (ensures fun h0 _ h1 ->
+    let b0 = Ghost.reveal b0 in
     let b1 = Ghost.reveal b1 in
     h0 == h1 /\ (model /\ crf a /\ h a b0 == h a b1 ==> b0 == b1))
 let injective a b0 b1 =
@@ -91,39 +93,43 @@ let injective a b0 b1 =
 /// a hash collision.  We should review this "flagless" style for
 /// crypto modelling.
 
-noextract 
+noextract
 private val stop: s:string -> Stack 'a
   (requires fun h -> True)
   (ensures fun h0 r h1 -> False)
 let rec stop (s:string) = stop s
 
-noextract 
-val hash: a:alg -> v:bytes -> Stack (tag a)
+// JP, NS: probably need to redo MDM to use modifies clauses; is Stack really
+// desired here or is ST ok? (note that MDM.extend could probably be redone to
+// use Stack instead of ST)
+noextract
+val hash: a:alg -> v:bytes -> ST (bytes_hash a)
   (requires fun h0 -> hashable v)
   (ensures fun h0 t h1 ->
-    LowStar.Buffer.(modifies loc_none h0 h1) /\
-    Seq.length v < maxLength a /\
-    t == h a v /\ 
+    LowStar.Buffer.(modifies (loc_region_only true tls_tables_region) h0 h1) /\
+    Seq.length v < max_input_length a /\
+    t == h a v /\
     hashed a v
   )
 
 open LowStar.Buffer
 
-module ST = FStar.HyperStack.ST 
+module ST = FStar.HyperStack.ST
 
 let hash a v =
-  let h0 = ST.get() in 
+  let h0 = ST.get() in
   assert_norm (pow2 61 < pow2 125);
-  assert(Seq.length v < maxLength a);
-  let t = Spec.Hash.hash a v in 
+  assert(Seq.length v < max_input_length a);
+  let t = Spec.Hash.hash a v in
   if crf a then (
     let x = Computed a t in
     match MDM.lookup table x with
       | None -> MDM.extend table x v
       | Some v' -> if v <> v' then stop "hash collision detected");
-  let h1 = ST.get() in 
+  let h1 = ST.get() in
+  assume LowStar.Buffer.(modifies (loc_region_only true tls_tables_region) h0 h1);
   //19-05-25 TODO stuck with an old library
-  assume(h0 == h1); //modifies loc_none h0 h1);
+  //assume(h0 == h1); //modifies loc_none h0 h1);
   t
 
 #set-options "--z3rlimit 100"
@@ -131,11 +137,11 @@ let hash a v =
 
 open FStar.Seq
 
-noextract 
+noextract
 private val test (a:alg {crf a}) (b0 b1: (b:bytes{hashable b})): St unit
 let test a b0 b1 =
-  let t0 = hash a b0 in 
+  let t0 = hash a b0 in
   let t1 = hash a b1 in
   injective a (Ghost.hide b0) (Ghost.hide b1);
   if model && t0 = t1 then assert(b0 == b1)
-  
+
